Get some more ARMv8 code with floats to decompile

examples/machine-code/graph/armv8_example/input/s.c
@@ -1,0 +1,55 @@
+double f(double x, double y)
+{
+	return x*y;
+}
+
+double g(double x, double y, double z)
+{
+	return x*y + z;
+}
+
+double h(double x)
+{
+	return x + 12.0;
+}
+
+double i(double x, double y)
+{
+	return x/y;
+}
+
+double j(double x, double y)
+{
+	return x + y;
+}
+
+double k(double x, double y)
+{
+	return x - y;
+}
+
+void m(void)
+{
+	__asm__ (
+		"str d0, [sp, #8]\n"
+		"str d1, [sp]\n"
+		"ldr d1, [sp, #8]\n"
+		"ldr d0, [sp]\n"
+		"fcmpe d1, d0\n"
+		"ldr d1, [sp, #8]\n"
+		"ldr d0, [sp]\n"
+		"fsub d0, d1, d0\n"
+		"str d0, [sp, #40]\n"
+		"ldr d0, [sp, #40]\n"
+		"fmov d1, x0\n"
+		"fadd d0, d0, d1\n"
+		"str d0, [sp, #48]\n"
+		"ldr d0, [sp, #40]\n"
+		"str d0, [sp, #32]\n"
+		"ldr d0, [sp, #48]\n"
+		"str d0, [sp, #32]\n"
+		"ldr d0, [sp, #32]\n"
+		"str d0, [sp, #56]\n"
+		"ldr d0, [sp, #56]\n"
+	);
+}
